Thread eta expansion everywhere (#676)
* Thread eta-expandedness assumptions through all the compilation passes

* Prove preservation of eta expanded fixpoints through erasure

* WIP fixing remaining eta-expansion glitches

* We need to eta-expand constructors as well to get preservation by let-expansion

* Produce properly eta-expanded contexts in inductive declarations

* Eta expansion preservation in PCUIC

* Show that Template to PCUIC preserve eta-expanded environments

* Refactor the various transformations so they live in their right place in Template/PCUIC/Erasure

* Refactor Erasure into multiple files, defining the structures, transfomations and the final pipeline

* Disable eta-expansion for now as it seems to produce ill-typed terms

* Add a template program that allows

* Add a metacoq program that allows to test well-typedness of expanded quoted programs.
This could be run systematically to perform translation-validation of the eta-expansion phase, but would be quite costly.

* Comment debug printing which can have very large output

* Fix build problem

* Fix safechecker

(cherry picked from commit 654f9a6acbadb6b11a533f778b4abd9893599c07)

template-coq/src/run_template_monad.ml
@@ -474,6 +474,7 @@ let rec run_template_program_rec ~poly ?(intactic=false) (k : Constr.t Plugin_co
   | TmUnquote t ->
     begin
        try
+         debug Pp.(fun () -> str"Unquoting:" ++ Printer.pr_constr_env env evm t);
          let t = reduce_all env evm t in
          let evm, t' = denote_term env evm t in
          let typ = Retyping.get_type_of env evm (EConstr.of_constr t') in
