erasure/theories/EDeps.v
@@ -785,3 +785,4 @@ Proof.
   eapply erases_deps_single; eauto.
   now eapply erases_global_all_deps.
 Qed.
+
