pcuic/theories/TemplateToPCUICExpanded.v
@@ -1,24 +1,195 @@
+From Equations Require Import Equations.
 From Coq Require Import ssreflect.
 From MetaCoq.Template Require Import config utils.
-From MetaCoq.Template Require Ast TypingWf WfAst TermEquality EtaExpand.
+From MetaCoq.Template Require Ast TypingWf WfAst TermEquality EtaExpand TemplateProgram.
 From MetaCoq.PCUIC Require Import PCUICAst PCUICAstUtils PCUICCumulativity
      PCUICLiftSubst PCUICEquality PCUICReduction 
      PCUICUnivSubst PCUICTyping PCUICGlobalEnv TemplateToPCUIC
-     PCUICWeakeningConv PCUICWeakeningTyp PCUICSubstitution PCUICGeneration PCUICCasesContexts TemplateToPCUICCorrectness PCUICEtaExpand.
+     PCUICWeakeningConv PCUICWeakeningTyp PCUICSubstitution PCUICGeneration 
+     PCUICCasesContexts TemplateToPCUICCorrectness PCUICEtaExpand
+     PCUICProgram.
+
 Tactic Notation "wf_inv" ident(H) simple_intropattern(p) :=
 (eapply WfAst.wf_inv in H; progress cbn in H; try destruct H as p) || 
 (apply WfAst.wf_mkApps_napp in H; [|easy]; try destruct H as p).
 
-
 Local Hint Constructors expanded : expanded.
+
+Lemma expanded_context_map2_bias_left Σ n bctx ctx :
+  #|ctx| = #|bctx| ->
+  expanded_context Σ n ctx ->
+  expanded_context Σ n
+     (map2_bias_left set_binder_name dummy_decl bctx ctx).
+Proof.
+  unfold expanded_context.
+  intros hl. 
+  rewrite map2_map2_bias_left //.
+  intros [a]. sq.
+  induction a in bctx, hl |- *; try econstructor; auto.
+  - cbn. destruct bctx; constructor.
+  - destruct bctx => //.
+    cbn. constructor; auto. cbn.
+    destruct (decl_body d); constructor => //. depelim p.
+    cbn in hl. assert (#|Γ| = #|bctx|) by lia.
+    rewrite map2_length //. now rewrite -H0.
+Qed.
+
+Import PCUICWeakeningEnvConv.
+
+Lemma extends_decls_trans Σ Σ' Σ'' : extends_decls Σ Σ' -> extends_decls Σ' Σ'' -> extends_decls Σ Σ''.
+Proof.
+  intros [? [ext ?]] [? [ext' ?]]. subst. split. now transitivity Σ'.
+  rewrite e0 in e2. exists (ext' ++ ext). now rewrite -app_assoc.
+Qed.
+
+Lemma declared_minductive_expanded Σ c mdecl :
+  expanded_global_env Σ ->
+  declared_minductive Σ c mdecl ->
+  exists Σ', ∥ extends_decls Σ' Σ ∥ /\ expanded_minductive_decl Σ' mdecl.
+Proof.
+  unfold expanded_global_env, declared_minductive, lookup_env.
+  destruct Σ as [univs Σ]; cbn.
+  intros exp; induction exp; cbn => //.
+  destruct decl as [kn d]; cbn.
+  destruct (eqb_spec c kn). intros [= ->].
+  subst c. eexists. split ; [|exact H]. sq. red. split => //. cbn. 
+  eexists. cbn. instantiate (1:= [_]); reflexivity.
+  intros hl; destruct (IHexp hl). exists x. intuition auto.
+  sq. eapply extends_decls_trans; tea. 
+  split => //. now exists [(kn, d)].
+Qed.
+
+Lemma declared_constructor_expanded {Σ c mdecl idecl cdecl} : 
+  expanded_global_env Σ ->
+  declared_constructor Σ c mdecl idecl cdecl ->
+  exists Σ', ∥ extends_decls Σ' Σ ∥ /\ expanded_minductive_decl Σ' mdecl /\ expanded_constructor_decl Σ' mdecl cdecl.
+Proof.
+  intros exp [[decli hnth] hnth'].
+  eapply declared_minductive_expanded in decli.
+  destruct decli as [Σ' [ext exp']]. exists Σ'; split => //. split => //.
+  destruct exp' as [hp hb]. solve_all. 
+  eapply nth_error_all in hb; tea.
+  destruct hb as [hb]. solve_all.
+  eapply nth_error_all in hb; tea.
+  auto.
+Qed.
+
+Lemma expanded_extended_subst {Σ Γ Δ} : 
+  expanded_context Σ Γ Δ -> 
+  forall n,
+  Forall (expanded Σ (repeat 0 (n + context_assumptions Δ) ++ Γ)) (extended_subst Δ n).
+Proof.
+  intros [a]; induction a. cbn. constructor.
+  cbn. destruct d as [na [b|] ty]; cbn in *. constructor; auto. 
+  { cbn. eapply (expanded_subst _ _ 0 _ []) => //. cbn. rewrite -/(repeat _ _).
+    specialize (IHa n). solve_all.
+    len. rewrite repeat_app Nat.add_comm. 
+    eapply expanded_lift. 1-2:now len; rewrite !repeat_length.
+    now depelim p. }
+  constructor; auto.
+  eapply (expanded_tRel _ _ _ _ []) => //. cbn.
+  rewrite nth_error_app_lt. rewrite repeat_length. lia.
+  rewrite nth_error_repeat //. lia.
+  specialize (IHa (S n)).
+  now rewrite Nat.add_succ_r.
+Qed.
+
+Lemma expanded_let_expansion {Σ} {Δ : context} {Γ t} :
+  expanded_context Σ Γ Δ ->
+  expanded_context Σ (repeat 0 #|Δ| ++ Γ) t ->
+  expanded_context Σ (repeat 0 (context_assumptions Δ) ++ Γ) (expand_lets_ctx Δ t).
+Proof.
+  rewrite /expanded_context.
+  intros [aΔ] [a]; sq.
+  unfold expand_lets_ctx, expand_lets_k_ctx.
+  do 2 eapply PCUICParallelReduction.All_fold_fold_context_k.
+  eapply All_fold_impl; tea. cbn.
+  intros Γ' x f. destruct (decl_body x) => //; constructor.
+  len. depelim f.
+  eapply expanded_subst. now rewrite repeat_length.
+  clear -aΔ. eapply (expanded_extended_subst (sq aΔ) 0).
+  len. rewrite app_assoc -repeat_app. eapply expanded_lift. len. now rewrite !repeat_length.
+  now rewrite repeat_length. rewrite repeat_app -app_assoc //.
+Qed.
+
+Lemma expanded_context_subst {Σ} {Δ Δ' : list nat} {Γ s k t} :
+  #|s| = #|Δ'| ->
+  #|Δ| = k ->
+  Forall (expanded Σ Γ) s ->
+  expanded_context Σ (Δ ++ repeat 0 #|Δ'| ++ Γ) t ->
+  expanded_context Σ (Δ ++ Γ) (subst_context s k t).
+Proof.
+  intros hs hs' has.
+  rewrite /expanded_context.
+  intros [aΔ]; sq.
+  eapply PCUICParallelReduction.All_fold_fold_context_k.
+  eapply All_fold_impl; tea. cbn.
+  intros Γ' x f. destruct (decl_body x) => //; constructor.
+  len. depelim f. rewrite app_assoc.
+  eapply expanded_subst. len. rewrite repeat_length. lia. solve_all. auto.
+  now rewrite -app_assoc hs.
+Qed.
+
+Lemma expanded_inds {Σ Γ ind u bodies} : Forall (expanded Σ Γ) (inds ind u bodies).
+Proof.
+  unfold inds. induction #|bodies|; cbn; auto. constructor => //. constructor.
+Qed.
+
+Implicit Types (cf : checker_flags).
+
+Lemma expanded_weakening {cf} {Σ Σ' Γ t} : 
+  wf Σ' -> extends_decls Σ Σ' -> expanded Σ Γ t -> expanded Σ' Γ t.
+Proof.
+  intros wfΣ ext.
+  eapply expanded_ind; intros.
+  all:try solve [econstructor; eauto].
+  - econstructor; eauto. solve_all. sq. eapply All_fold_impl; tea; cbn.
+    intros ? ? []; constructor; auto. now rewrite <- repeat_app.
+  - eapply expanded_tConstruct_app; tea.
+    eapply weakening_env_declared_constructor; tea. now eapply extends_decls_extends.
+Qed.
+
+Lemma expanded_context_weakening {cf} {Σ Σ' Γ t} : 
+  wf Σ' -> extends_decls Σ Σ' -> expanded_context Σ Γ t -> expanded_context Σ' Γ t.
+Proof.
+  intros wfΣ ext.
+  intros [a]; sq.
+  eapply All_fold_impl; tea; cbn; eauto.
+  intros ?? []; constructor.
+  now eapply expanded_weakening.
+Qed.
+
+Lemma expanded_bcontext {cf} Σ ind k mdecl idecl cdecl bctx bbody :
+  wf Σ ->
+  PCUICEtaExpand.expanded_global_env Σ ->
+  #|cstr_branch_context ind mdecl cdecl| = #|bctx| ->
+  declared_constructor Σ (ind, k) mdecl idecl cdecl ->
+  expanded_context Σ (repeat 0 (context_assumptions mdecl.(ind_params))) (bcontext (trans_branch ind mdecl cdecl bctx bbody)).
+Proof.
+  intros wfΣ expΣ hl declc.
+  eapply expanded_context_map2_bias_left => //.
+  destruct (declared_constructor_expanded expΣ declc) as [Σ' [ext [expm expc]]].
+  destruct expm as [hp hb]. destruct expc as [hargs].
+  unfold cstr_branch_context.
+  epose proof (expanded_let_expansion hp (t:=(subst_context
+  (inds (inductive_mind ind) (abstract_instance (ind_universes mdecl))
+     (ind_bodies mdecl)) #|ind_params mdecl| 
+  (cstr_args cdecl)))).
+  rewrite !app_nil_r in H. forward H.
+  epose proof (expanded_context_subst (Γ := []) (Δ' := repeat 0 #|ind_bodies mdecl|)).
+  rewrite !app_nil_r in H0. eapply H0; rewrite ?repeat_length //. len. apply expanded_inds.
+  rewrite -repeat_app. exact hargs.
+  destruct ext. eapply expanded_context_weakening; tea.
+Qed.
 
 Lemma trans_expanded {cf : checker_flags} {Σ} {wfΣ : Template.Typing.wf Σ} Γ T  :
   let Σ' := trans_global_env Σ in
   WfAst.wf Σ T ->
+  PCUICEtaExpand.expanded_global_env Σ' ->
   EtaExpand.expanded Σ Γ T ->
   expanded Σ' Γ (trans Σ' T).
 Proof with eauto using expanded.
-  intros Σ' wf exp. revert wf.
+  intros Σ' wf expΣ' exp. revert wf.
   induction exp; intros wf; cbn -[Σ']...
   all: try now (wf_inv wf []; eauto using expanded).
   - wf_inv wf ?. eapply expanded_tRel with (args := []). eauto. lia. econstructor.
@@ -38,9 +209,20 @@ Proof with eauto using expanded.
   - wf_inv wf (mdecl' & idecl' & []). eapply forall_decls_declared_inductive in d; eauto. 2: now eapply template_to_pcuic_env.
     unfold Σ'.
     erewrite trans_lookup_inductive, declared_inductive_lookup; eauto.
-    econstructor; eauto. cbn. induction a1; cbn; econstructor.
-    + cbn. inversion H0; subst. rewrite map2_bias_left_length. len. eapply H3. eapply r.
-    + inversion H0; subst. inversion H; subst. eapply IHa1; eauto.
+    econstructor; eauto. cbn.
+    + solve_all.
+    + cbn. eapply All2_nth_hyp in a1.
+      eapply All_Forall, All2_All_map2, All2_map.
+      eapply Forall_All in H2. eapply All2_All_mix_right in a1; tea.
+      eapply All2_impl; tea. intros x y. cbv beta. intros [[i [Hi []]] ?].
+      split.
+      { rewrite map_length. relativize #|Ast.pparams type_info|.
+        eapply expanded_bcontext => //.
+        - now eapply template_to_pcuic_env.
+        - len. eapply All2_length in a2. len in a2.
+        - split; tea. cbn; rewrite nth_error_map. erewrite Hi => //.
+        - cbn. tea. rewrite context_assumptions_map. now rewrite e. }
+      * cbn. rewrite map2_bias_left_length. now eapply e0.
     + eapply template_to_pcuic_env; eauto.
   - now (wf_inv wf [[]]; eauto using expanded).
   - wf_inv wf [[]]. wf_inv w ?. eapply expanded_tFix.
@@ -52,4 +234,140 @@ Proof with eauto using expanded.
   - wf_inv wf ?. econstructor. solve_all.
   - wf_inv wf [[[]]]. eapply forall_decls_declared_constructor in H; eauto. 2: now eapply template_to_pcuic_env.
     eapply expanded_tConstruct_app. eauto. cbn. unfold trans_local. now rewrite map_length context_assumptions_map. solve_all.
+Qed.
+
+
+Lemma wf_cons_inv {cf} univs (Σ : global_declarations) d : wf {| universes := univs; declarations := d :: Σ |} -> wf {| universes := univs; declarations := Σ |}.
+Proof.
+  intros []. split => //. now depelim o0.
+Qed.
+
+Lemma template_wf_cons_inv {cf} univs (Σ : Ast.Env.global_declarations) d : Typing.wf {| Ast.Env.universes := univs; Ast.Env.declarations := d :: Σ |} ->
+  let Σ' := {| Ast.Env.universes := univs; Ast.Env.declarations := Σ |} in
+  Typing.wf Σ' × Typing.on_global_decl (WfAst.wf_decl_pred) (Σ', Ast.universes_decl_of_decl d.2) d.1 d.2
+  × ST.on_udecl univs (Ast.universes_decl_of_decl d.2).
+Proof.
+  intros wf; split.
+  destruct wf. split => //. now depelim o0.
+  eapply typing_wf_wf in wf. depelim wf.
+  cbn in o0. depelim o0. cbn. split => //.
+  eapply TypingWf.on_global_decl_impl; tea. cbn.
+  intros. destruct T => //. red. red in X0. destruct X0. intuition auto.
+  cbn. split => //.
+Qed.
+
+Lemma trans_global_env_cons univs (Σ : Ast.Env.global_declarations) decl : 
+  trans_global_env {| S.Env.universes := univs; S.Env.declarations := decl :: Σ |} = 
+  let Σ' := trans_global_env {| S.Env.universes := univs; S.Env.declarations := Σ |} in 
+  add_global_decl Σ' (decl.1, trans_global_decl Σ' decl.2). 
+Proof. reflexivity. Qed.
+
+Arguments trans_global_env : simpl never.
+
+Lemma eta_global_env Σ : Σ = {| universes := Σ.(universes); declarations := Σ.(declarations) |}.
+Proof. now destruct Σ. Qed.
+
+Lemma eta_template_global_env Σ : Σ = {| S.Env.universes := Σ.(S.Env.universes); S.Env.declarations := Σ.(S.Env.declarations) |}.
+Proof. now destruct Σ. Qed.
+
+Lemma All_fold_map (P : context -> context_decl -> Type) (f : Ast.Env.context_decl -> context_decl) ctx :
+  All_fold P (map f ctx) <~> All_fold (fun Γ d => P (map f Γ) (f d)) ctx.
+Proof.
+  induction ctx.
+  - split; constructor.
+  - cbn. split; intros H; depelim H; constructor; auto; now apply IHctx.
+Qed.
+
+Lemma All_fold_All_mix_left (P : S.Env.context -> S.Env.context_decl -> Type) (Q : S.Env.context_decl -> Type) ctx :
+  All_fold P ctx -> 
+  All Q ctx ->
+  All_fold (fun Γ d => Q d × P Γ d) ctx.
+Proof.
+  induction 1; cbn; intros. constructor.
+  depelim X0. constructor; auto.
+Qed.
+
+Lemma expanded_trans_local {cf} {Σ} {wfΣ : Typing.wf Σ} Γ ctx : 
+  expanded_global_env (trans_global_env Σ) ->
+  All (WfAst.wf_decl Σ) ctx ->
+  EtaExpand.expanded_context Σ Γ ctx -> 
+  expanded_context (trans_global_env Σ) Γ (trans_local (trans_global_env Σ) ctx).
+Proof.
+  rewrite /expanded_context.
+  intros etaΣ wfctx [a]; split.
+  unfold trans_local.
+  eapply All_fold_map.
+  eapply All_fold_All_mix_left in a; tea.
+  eapply All_fold_impl; tea; cbv beta; intros ??; cbn; unfold WfAst.wf_decl; 
+    intros [wf Hd]; revert Hd wf; intros []; intros [];  constructor; len.
+  eapply trans_expanded in H; auto.
+Qed.
+
+Lemma wf_context_sorts {cf} {Σ ctx ctx' cunivs} {wfΣ : Typing.wf_ext Σ} :
+  Typing.sorts_local_ctx WfAst.wf_decl_pred Σ ctx ctx' cunivs -> 
+  All (WfAst.wf_decl Σ) ctx'.
+Proof.
+  induction ctx' in cunivs |- *; cbn; auto.
+  destruct a as [na [b|] ty].
+  intros [? []]. constructor; auto. eauto.
+  destruct cunivs => //.
+  intros [? []]. constructor; eauto. constructor; cbn; eauto.
+Qed.
+  
+Lemma expanded_trans_global_env {cf} Σ {wfΣ : Typing.wf_ext Σ} :
+  EtaExpand.expanded_global_env Σ ->
+  expanded_global_env (trans_global_env Σ).
+Proof. 
+  destruct Σ as [[univs Σ] udecl]. 
+  cbn -[trans_global_env]. unfold EtaExpand.expanded_global_env; cbn -[trans_global_env].
+  intros etaenv; induction etaenv.
+  - constructor; auto.
+  - destruct wfΣ as [wfΣ onudecl].
+    eapply template_wf_cons_inv in wfΣ as [].
+    forward IHetaenv by tea. split => //.
+    rewrite trans_global_env_cons. set (Σ' := trans_global_env _ ).
+    cbv zeta. constructor. apply IHetaenv.
+    cbn -[add_global_decl trans_global_env].
+    destruct decl as [kn []]; cbn in *; depelim H => //.
+    * unfold trans_constant_body; cbn.
+      constructor. cbn. destruct p.
+      red in o.
+      destruct (Ast.Env.cst_body c); cbn => //. cbn in expanded_body.
+      eapply trans_expanded in expanded_body; eauto.
+      rewrite -/Σ' in expanded_body. now rewrite -eta_global_env.
+      red in o. now destruct o.
+    * rewrite -eta_global_env.
+      constructor.
+      + cbn. eapply expanded_trans_local in expanded_params => //.
+        destruct p; destruct o. now eapply TypingWf.All_local_env_wf_decls.
+      + cbn. destruct p.
+        move: o.(Typing.onInductives). destruct o. intros oni.
+        eapply All_Forall. eapply Forall_All in expanded_ind_bodies.
+        eapply Alli_All_mix in oni; tea. clear expanded_ind_bodies.
+        eapply All_map, Alli_All; tea; cbv beta.
+        intros n oib []. move: (Typing.onConstructors o).
+        intros onc. red in onc.
+        destruct e as [expc]. constructor. eapply Forall_All in expc.
+        eapply All2_All_mix_left in onc; tea. clear expc. solve_all.
+        cbn. solve_all.
+        destruct a as [expargs expty]. constructor.
+        { cbn. eapply expanded_trans_local in expargs; eauto.
+          move: expargs. len.
+          move: b.(Typing.on_cargs) => onargs.
+          eapply @wf_context_sorts in onargs; tea.
+          cbn. split => /= //. exact w. }
+Qed.
+
+Import TemplateProgram.
+
+Lemma expanded_trans_program {cf : checker_flags} p (t : wt_template_program p) :
+  EtaExpand.expanded_program p ->
+  expanded_pcuic_program (trans_template_program p).
+Proof.
+  intros [etaenv etat].
+  destruct t as [? [T HT]]. split.
+  unshelve eapply expanded_trans_global_env => //; tc.
+  unshelve eapply trans_expanded => //; tc. eapply w.
+  now unshelve eapply TypingWf.typing_wf in HT.
+  eapply expanded_trans_global_env => //.
 Qed.
