template-coq/theories/TemplateCheckWf.v
@@ -1,0 +1,75 @@
+From Coq Require Import List.
+From MetaCoq.Template Require Import config Transform TemplateProgram Pretty All Loader.
+Import ListNotations.
+Import MCMonadNotation.
+Import bytestring.
+Open Scope bs_scope.
+
+#[local] Existing Instance config.default_checker_flags.
+
+Definition run_eta_program := Transform.run template_eta_expand.
+
+Definition eta_expand p := 
+  run_eta_program p (todo "assume well-typedness").
+
+Definition check_def (d : kername × global_decl) : TemplateMonad unit :=
+  match d.2 with
+  | ConstantDecl cb =>
+    match cb.(cst_body) with
+    | Some body => 
+      tmMsg ("Unquoting eta-expanded " ++ string_of_kername d.1)%bs ;;
+      tmUnquote body ;;
+      tmMsg ("Succeeded")
+    | None => ret tt
+    end
+  | InductiveDecl idecl => ret tt
+  end.
+
+Definition is_nil {A} (l : list A) :=
+  match l with
+  | [] => true
+  | _ :: _ => false
+  end.
+
+Fixpoint wfterm (t : term) : bool :=
+  match t with
+  | tRel i => true
+  | tEvar ev args => List.forallb (wfterm) args
+  | tLambda _ T M | tProd _ T M => wfterm T && wfterm M
+  | tApp u v => wfterm u && List.forallb (wfterm) v && negb (isApp u) && negb (is_nil v)
+  | tCast c kind t => wfterm c && wfterm t
+  | tLetIn na b t b' => wfterm b && wfterm t && wfterm b'
+  | tCase ind p c brs =>
+    let p' := test_predicate (fun _ => true) (wfterm) (wfterm) p in
+    let brs' := forallb (wfterm ∘ bbody) brs in
+    p' && wfterm c && brs'
+  | tProj p c => wfterm c
+  | tFix mfix idx =>
+    List.forallb (test_def wfterm wfterm) mfix
+  | tCoFix mfix idx =>
+    List.forallb (test_def wfterm wfterm) mfix
+  | _ => true
+  end.
+
+From Coq Require Import ssrbool.
+
+Definition wf_global_decl d := 
+  match d with
+  | ConstantDecl cb => wfterm cb.(cst_type) && option_default wfterm cb.(cst_body) true
+  | InductiveDecl idecl => true
+  end.
+Definition wf_global_declarations : global_declarations -> bool := forallb (wf_global_decl ∘ snd).
+Definition wf_global_env (g : global_env) := wf_global_declarations g.(declarations).
+Definition wf_program p := wf_global_env p.1 && wfterm p.2.
+
+Definition check_wf (g : Ast.Env.program) : TemplateMonad unit :=
+  monad_map check_def g.1.(declarations) ;; 
+  tmMsg "Wellformed global environment" ;; ret tt.
+  
+Definition check_wf_eta (g : Ast.Env.program) : TemplateMonad unit :=
+  monad_map check_def (eta_expand g).1.(declarations) ;; 
+  tmMsg "Wellformed eta-expanded global environment" ;; ret tt.
+
+(* To test that a program's eta-expansion is indeed well-typed according to Coq's kernel use: 
+ 
+  MetaCoq Run (tmQuoteRec wf_program >>= check_wf_eta). *)
