template-coq/theories/Transform.v
@@ -1,0 +1,91 @@
+(* Distributed under the terms of the MIT license. *)
+
+(** Generic transofmations from one language to another, 
+    preserving an evaluation relation up-to some observational equality. *)
+
+From Coq Require Import Program ssreflect ssrbool.
+From Equations Require Import Equations.
+From MetaCoq.Template Require Import utils.
+Import bytestring.
+Local Open Scope bs.
+Local Open Scope string_scope2.
+
+(* Used to show timings of the ML execution *)
+ 
+Definition time : forall {A B}, string -> (A -> B) -> A -> B :=
+  fun A B s f x => f x.
+
+Extract Constant time => 
+  "(fun c f x -> let s = Caml_bytestring.caml_string_of_bytestring c in Tm_util.time (Pp.str s) f x)".
+
+Module Transform.
+  Section Opt.
+     Context {program program' : Type}.
+     Context {value value' : Type}.
+     Context {eval :  program -> value -> Prop}.
+     Context {eval' : program' -> value' -> Prop}.
+     
+     Definition preserves_eval pre (transform : forall p : program, pre p -> program') obseq :=
+      forall p v (pr : pre p),
+        eval p v ->
+        let p' := transform p pr in
+        exists v', eval' p' v' /\ obseq p p' v v'.
+
+    Record t := 
+    { name : string; 
+      pre : program -> Prop; 
+      transform : forall p : program, pre p -> program';
+      post : program' -> Prop;
+      correctness : forall input (p : pre input), post (transform input p);
+      obseq : program -> program' -> value -> value' -> Prop;
+      preservation : preserves_eval pre transform obseq; }.
+
+    Definition run (x : t) (p : program) (pr : pre x p) : program' := 
+      time x.(name) (fun _ => x.(transform) p pr) tt.
+
+  End Opt.
+  Arguments t : clear implicits.
+
+  Definition self_transform program value eval eval' := t program program value value eval eval'.
+
+  Section Comp.
+    Context {program program' program'' : Type}.
+    Context {value value' value'' : Type}.
+    Context {eval : program -> value -> Prop}.
+    Context {eval' : program' -> value' -> Prop}.
+    Context {eval'' : program'' -> value'' -> Prop}.
+    
+    Local Obligation Tactic := idtac.
+    Program Definition compose (o : t program program' value value' eval eval') (o' : t program' program'' value' value'' eval' eval'') 
+      (hpp : (forall p, o.(post) p -> o'.(pre) p)) : t program program'' value value'' eval eval'' :=
+      {| 
+        name := (o.(name) ^ " -> " ^ o'.(name))%bs;
+        transform p hp := run o' (run o p hp) (hpp _ (o.(correctness) _ hp));
+        pre := o.(pre);
+        post := o'.(post);
+        obseq g g' v v' := exists g'' v'', o.(obseq) g g'' v v'' × o'.(obseq) g'' g' v'' v'
+        |}.
+    Next Obligation.
+      intros o o' hpp inp pre.
+      eapply o'.(correctness).
+    Qed.
+    Next Obligation.
+      red. intros o o' hpp.
+      intros p v pr ev.
+      eapply (o.(preservation) _ _ pr) in ev; auto.
+      cbn in ev. destruct ev as [v' [ev]].
+      epose proof (o'.(preservation) (o.(transform) p pr) v').
+      specialize (H0 (hpp _ (o.(correctness) _ pr)) ev).
+      destruct H0 as [v'' [ev' obs']].
+      exists v''. constructor => //.
+      exists (transform o p pr), v'. now split.
+    Qed.
+  End Comp.
+
+  Declare Scope transform_scope.
+  Bind Scope transform_scope with t.
+
+  Notation " o ▷ o' " := (Transform.compose o o' _) (at level 50, left associativity) : transform_scope.
+
+  Open Scope transform_scope.
+End Transform.
